\documentclass[fleqn]{article}
\usepackage{amsmath}
\usepackage{amssymb}
\usepackage[parfill]{parskip}
\usepackage[vmargin=0.5cm]{geometry}
\setlength\parindent{0pt}
\setlength{\mathindent}{0pt}
\begin{document}
\begin{align*}
  \text{Let } S_{k} = \text{all sets $T$ of the form }
                      \lbrace x' : & 1 \leq x \leq n \\
                                   & x \in \mathbb{Z} \\
                                   & \text{Let } x' = \pm x^2 \\
                                   & -x' \not\in T
                      \rbrace
\end{align*}
for positive integer $k$ and some positive integer $n$, such that:\\
$\displaystyle\sum\limits_{z \in T} z = k \wedge  |T| = n$.

Let $P(k)$ be true $\Leftrightarrow S_{k} \not= \emptyset $.

Proof of $P$ by Induction on $k$

Base Cases:\\
$k = 1:$\\
Let $T = \lbrace 1 \rbrace$.\\
$\displaystyle\sum\limits_{z \in T} z = 1 \Rightarrow
T \in S_{1} \Rightarrow P(1)$.

$k = 2:$\\
Let $T = \lbrace -1,-4,-9,16 \rbrace$.\\
$\displaystyle\sum\limits_{z \in T} z = 2 \Rightarrow 
T \in S_{2} \Rightarrow P(2)$.

$k = 3:$\\
Let $T = \lbrace-1,4\rbrace$.\\
$\displaystyle\sum\limits_{z \in T} z = 3 \Rightarrow 
T \in S_{3} \Rightarrow P(3)$.

$k = 4:$\\
Let $T = \lbrace -1,-4,9 \rbrace$.\\
$\displaystyle\sum\limits_{z \in T} z = 4 \Rightarrow 
T \in S_{4} \Rightarrow P(4)$.

Inductive Case: Let $k \geq 1$.\\
Assume $P(k)$ is true.\\
WTS $P(k) \Rightarrow P(k+4)$ is true.\\
Firstly, we'd like to show that for all positive integers $n$, \\
Lemma 1: $n^2 - (n+1)^2 - (n+2)^2 + (n+3)^2 = 4$\\
Let $n \in \mathbb{N}$.\\
$n^2 - (n+1) ^2 - (n+2)^2 + (n+3)^2 =\\
n^2 - (n^2 + 2n + 1) - (n^2 + 4n + 4) + (n^2 + 6n + 9) =\\
n^2 - n^2 - 2n - 1 - n^2 - 4n - 4 + n^2 + 6n + 9 = \\
4 $

Since $P(k)$ is true, $\Rightarrow S_{k} \not= \emptyset$\\
Take $S'$ from $S_{k}$.\\
Let $m^2 = max(\lbrace |x| : x \in S_{k} \rbrace)$\\
Let $M = \lbrace (m+1)^2, -(m+2)^2, -(m+3)^2, (m+4)^2 \rbrace$\\
By the definition of $m^2$ and $S'$, clearly $S' \cap M = \emptyset$\\
Let $T = S' \cup M \\$
Visibly, $|T| = m+4 \wedge 
         \forall 1 \leq x \leq m+4, x \in \mathbb{Z} \Rightarrow
                                    x^2 \in T \veebar -x^2 \in T\\$
\begin{align*}
  \displaystyle\sum\limits_{z \in T} z 
  &=\displaystyle\sum\limits_{z \in S'} z + \displaystyle\sum\limits_{z \in M} z, \text{which by $P(k)$ }\\
  &=k + \displaystyle\sum\limits_{z \in M} z,\text{which by Lemma 1 }\\
  &=k + 4 = \displaystyle\sum\limits_{z \in T} z \\
  &\Rightarrow T \in S_{k+4}\\
  &\Rightarrow P(k+4).
\end{align*}
By mathematical induction, $P$ is true.

\end{document}
